
(A + B) x C = (A x C) + (B x C)

(X, X') (x) (Y, Y') = (X x Y, X' x Y')
(X, X') x (Y, Y') = (X x Y, X' + Y')
(X, Z) + (Y, Z) = (X + Y, Z)

((A, Z) + (B, Z)) (x) (C, C') 
= (A + B, Z) (x) (C, C')
= ((A + B) x C, Z x C')
= ((A x C) + (B x C), Z x C')
= (A x C, Z x C') + (B x C, Z x C')
= ((A, Z) (x) (C, C')) + ((B, Z) (x) (C, C'))
** Yes

((A, Z) + (B, Z)) x (C, C')
= (A + B, Z) x (C, C')
= ((A + B) x C, Z + C')
= ((A x C) + (B x C), Z + C')
= (A x C, Z + C') + (B x C, Z + C')
= ((A, Z) x (C, C')) + ((B, Z) x (C, C'))
** Yes

((A, A') x (B, B')) (x) (C, C')
= (A x B, A' + B') (x) (C, C')
= (A x B x C, (A' + B') x C')
= (A x B x C, (A' x C') + (B' x C'))
** No - linearly distributive? Directed with copy?
